% !TeX program = lualatex

% Copyright (c) 2020-2025 Simon Crase

% Permission is hereby granted, free of charge, to any person obtaining a copy
% of this software and associated documentation files (the "Software"), to deal
% in the Software without restriction, including without limitation the rights
% to use, copy, modify, merge, publish, distribute, sublicense, and/or sell
% copies of the Software, and to permit persons to whom the Software is
% furnished to do so, subject to the following conditions:

% The above copyright notice and this permission notice shall be included in all
% copies or substantial portions of the Software.

% THE SOFTWARE IS PROVIDED "AS IS", WITHOUT WARRANTY OF ANY KIND, EXPRESS OR
% IMPLIED, INCLUDING BUT NOT LIMITED TO THE WARRANTIES OF MERCHANTABILITY,
% FITNESS FOR A PARTICULAR PURPOSE AND NONINFRINGEMENT. IN NO EVENT SHALL THE
% AUTHORS OR COPYRIGHT HOLDERS BE LIABLE FOR ANY CLAIM, DAMAGES OR OTHER
% LIABILITY, WHETHER IN AN ACTION OF CONTRACT, TORT OR OTHERWISE, ARISING FROM,
% OUT OF OR IN CONNECTION WITH THE SOFTWARE OR THE USE OR OTHER DEALINGS IN THE
% SOFTWARE.

\documentclass[]{article}
\usepackage{caption}
\usepackage{subcaption}
\usepackage{graphicx}
\usepackage{float}
\usepackage{url}
\usepackage{amsmath}
\usepackage{amssymb}
\usepackage{amsthm}
\usepackage{tocloft}
\usepackage{cancel}
\usepackage{thmtools}
\usepackage{gensymb}
\usepackage{braket}
\usepackage{bm}
\usepackage[compat=1.1.0]{tikz-feynman}
\usepackage{tikz}
\usepackage{pgfplots}
\usepackage{mathtools}
\usepackage{color}
\usepackage{colortbl}
\usepackage[toc,nonumberlist]{glossaries}
\usepackage{glossaries-extra}
\usepackage{mathtools}

\newcommand\numberthis{\addtocounter{equation}{1}\tag{\theequation}}

\newtheorem{thm}{Theorem}
\newtheorem{defn}[thm]{Definition}
\newtheorem{cor}[thm]{Corollary}
\newtheorem{lemma}[thm]{Lemma}
\graphicspath{{figs/}}
\widowpenalty10000
\clubpenalty10000
\setcounter{tocdepth}{2}
\tikzfeynmanset{compat=1.1.0}
\definecolor{Gray}{gray}{0.5}
\DeclareMathOperator{\Tr}{Tr \;}
\newcommand{\Lagr}{\mathcal{L}}
\renewcommand{\thesection}{2.\arabic{section}}
\setlength{\cftsubsecindent}{0em}
\setlength{\cftsecnumwidth}{3em}
\setlength{\cftsubsecnumwidth}{3em}
%opening
\title{Quantum Field Theory\\
Part II: Dirac and the Spinor}
\author{Simon Crase (compiler)\\simon@greenweaves.nz}

\begin{document}

\maketitle

\begin{abstract}

This document contains derivations of equations from \cite[Part II: Dirac and the Spinor]{zee2010quantum}.

\end{abstract}

\tableofcontents

\section{The Dirac Equation}

\begin{align*}
	(i\gamma^\mu\partial_\mu-m)\psi=&0\\
	\implies&\\
	(i\gamma^\mu\partial_\mu+m)(i\gamma^\nu\partial_\nu-m)\psi=&0 \\
	\iff&\\
	\big(-\gamma^\mu\partial_\mu\gamma^\nu\partial_\nu+\cancel{m i\gamma^\nu\partial_\nu}-\cancel{mi\gamma^\mu\partial_\mu}-m^2\big)\psi=&0\\
	\iff&\\
	\big(\gamma^\mu\partial_\mu\gamma^\nu\partial_\nu+m^2\big)\psi=&0\\
	\iff&\\
	\big(\gamma^\mu\gamma^\nu\partial_\mu\partial_\nu+m^2\big)\psi=&0\\
	\iff&\\
	\big[(\frac{1}{2}(\gamma^\mu\gamma^\nu+\gamma^\nu\gamma^\mu)\partial_\mu\partial_\nu+m^2\big]\psi=&0\\
	\text{Define} \{\gamma^\mu,\gamma^\nu\}=\gamma^\mu\gamma^\nu+\gamma^\nu\gamma^\mu\.\iff&\\
	\big(\frac{1}{2}\{\gamma^\mu,\gamma^\nu\}\partial_\mu\partial_\nu+m^2\big)\psi=&0\\
	\text{setting } \{\gamma^\mu,\gamma^\nu\}=2\eta^{\mu\nu}\.\implies&\\
	(\partial^2 + m^2)\psi =& 0
\end{align*}
\cite{zee2010quantum} defines the $\gamma$s in terms of the Pauli matrices $\sigma/\tau$:
\begin{align*}
	\gamma^0 =& I \otimes \tau_3\\
	\gamma^j =& i \sigma^j \otimes \tau_2
\end{align*}

\subsection{Cousins of the Gamma Matrices}
We collect some properties of the Pauli matrices.
\begin{align*}
	\sigma^x =& \begin{bmatrix} \numberthis \label{eq:pauli:x}
		0&1\\
		1&0
	\end{bmatrix}\\
	\sigma^y =& \begin{bmatrix} \numberthis \label{eq:pauli:y}
		0&-i\\
		i&0
	\end{bmatrix}\\
	\sigma^z =& \begin{bmatrix} \numberthis \label{eq:pauli:z}
		1&0\\
		0&-1
	\end{bmatrix}\\
	\sigma^x \sigma^y \sigma^z =& \begin{bmatrix} 
		0&1\\
		1&0
	\end{bmatrix} \begin{bmatrix} 
		0&-i\\
		i&0
	\end{bmatrix}\begin{bmatrix} 
		1&0\\
		0&-1
	\end{bmatrix}\\
	=& \begin{bmatrix}
		i&0\\
		0&-i\\
	\end{bmatrix}\begin{bmatrix} 
		1&0\\
		0&-1
	\end{bmatrix}\\
	=& i I
\end{align*}

The Dirac gamma matrices have the following representation.
\begin{align*}
	\gamma^0 =& \begin{bmatrix} \numberthis \label{eq:gamma:0}
	I&0\\
	0&-I
\end{bmatrix}\\
\gamma^i =& \begin{bmatrix}  \numberthis \label{eq:gamma:i}
	0&\sigma^i\\
	-\sigma^i&0
\end{bmatrix}	
\end{align*}

From \cite[II.1,(2)]{zee2010quantum}
\begin{align*}
	\{\gamma^\mu,\gamma^\nu\}=&2\eta^{\mu\nu} \numberthis \label{eq:gamma:anti}\\
	\{\gamma^0,\gamma^0\}=&2\eta^{00}\\
	\gamma^0\gamma^0=&I  \numberthis \label{eq:gamma:00}\\
	\{\gamma^i,\gamma^i\}=&2\eta^{ii}\\
	\gamma^i\gamma^i=&-I	 \numberthis \label{eq:gamma:ii}
\end{align*}
Expanding \eqref{eq:gamma:anti}
\begin{align*} 
	\gamma^\mu\gamma^\nu + \gamma^\nu\gamma^\mu=&2\eta^{\mu\nu}\\
	\gamma^\mu\gamma^\nu =& \eta^{\mu\nu} + \eta^{\mu\nu} -\gamma^\nu\gamma^\mu\\
	=&\eta^{\mu\nu}-i\sigma^{\mu\nu} \text{, where}\\
	\sigma^{\mu\nu}=&i \big(\eta^{\mu\nu} -\gamma^\nu\gamma^\mu\big) \text{. Now apply \eqref{eq:gamma:anti} again}\\
	=&i\big(\frac{1}{2}(\gamma^\mu\gamma^\nu + \gamma^\nu\gamma^\mu)-\gamma^\nu\gamma^\mu\big)\\
	=&i\big(\frac{1}{2}(\gamma^\mu\gamma^\nu - \gamma^\nu\gamma^\mu)\big)\\
	=&\frac{i}{2}[\gamma^\mu,\gamma^\nu]
\end{align*}

From \cite[II,(7)]{zee2010quantum}
\begin{align*}
	\gamma^5 =& i \gamma^0 \gamma^1 \gamma^2 \gamma^3 \numberthis \label{eq:gamma:5}
\end{align*}

Using the representation \eqref{eq:gamma:0} and \eqref{eq:gamma:i}.
\begin{align*}
	\gamma^5=& i \begin{bmatrix}
		I&0\\
		0&-I
	\end{bmatrix} \begin{bmatrix}
		0&\sigma^1\\
		-\sigma^1&0
	\end{bmatrix} \begin{bmatrix}
		0&\sigma^2\\
		-\sigma^2&0
	\end{bmatrix} \begin{bmatrix}
		0&\sigma^3\\
		-\sigma^3&0
	\end{bmatrix}\\
	=& i \begin{bmatrix}
		0&\sigma^1\\
		\sigma^1&0
	\end{bmatrix} \begin{bmatrix*}
		-\sigma^2 \sigma^3&0\\
		0&-\sigma^2 \sigma^3
	\end{bmatrix*}\\
	=& i \begin{bmatrix}
		0&-\sigma^1 \sigma^2 \sigma^3\\
		-\sigma^1 \sigma^2 \sigma^3&0
	\end{bmatrix}\\
	=& \begin{bmatrix}
		0&I\\
		I&0
	\end{bmatrix}
\end{align*}
Which agrees with \cite[II,(8)]{zee2010quantum}.
\begin{align*}
	\gamma^0 (\gamma^1 \gamma^2 \gamma^3) =& -i \gamma^5\\
	(\gamma^0)^2 (\gamma^1 \gamma^2 \gamma^3) =& -i \gamma^0 \gamma^5\\
	I \gamma^1 \gamma^2 \gamma^3 =& -i \gamma^0 \gamma^5\\
	\gamma^1 \gamma^2 \gamma^3 =& -i \gamma^0 \gamma^5
\end{align*}

From \eqref{eq:gamma:anti}:
\begin{align*}
	\gamma^0 \gamma_i =& \eta^{0i}-\gamma^i \gamma^0\\
	=& - \gamma^i\gamma^0 \text{, so \eqref{eq:gamma:5} becomes:}\\
	\gamma^5 =& - i \gamma^1 \gamma^0 \gamma^2 \gamma^3\\
	\gamma^1 \gamma^5 =& - i (\gamma^1)^2 \gamma^0 \gamma^2 \gamma^3\\
	i \gamma^0 \gamma^2 \gamma^3 =&\gamma^1 \gamma^5 \text{, from \eqref{eq:gamma:ii}}\\
	\gamma^0 \gamma^2 \gamma^3 =&-i\gamma^1 \gamma^5\\
\end{align*}

\subsection{Isomorphism $\frac{SU(2)}{Z^2} \cong SO(3)$}


In \cite[Section 3]{westra2008SU2} a $2\times 2$ unimodular unitary matrix has the form:
\begin{align*}
	U =& \begin{bmatrix}
		x&-y\\
		\bar{y}&\bar{x}
	\end{bmatrix} \text{. Substituting}\\
	x =& \cos{\theta} e^{i\phi}, \; y = \sin{\theta} e^{i\psi} \numberthis \label{eq:xy} \text{, gives} \\
	U=& \begin{bmatrix}
		\cos{\theta} e^{i\phi}&\sin{\theta}e^{i\psi}\\
		-sin{\theta}e^{-i\psi}&\cos{\theta} e^{-i\phi}
	\end{bmatrix}\\
	U^T =& \begin{bmatrix}
		\cos{\theta} e^{-i\phi}&-\sin{\theta}e^{i\psi}\\
		sin{\theta}e^{-i\psi}&\cos{\theta} e^{i\phi}
	\end{bmatrix}
\end{align*}
We follow \cite[Section 4]{westra2008SU2} and transform the Pauli Matrices.
\begin{align*}
	U \sigma^1 U^T  =&  \begin{bmatrix}
		\cos{\theta} e^{i\phi}&\sin{\theta}e^{i\psi}\\
		-\sin{\theta}e^{-i\psi}&\cos{\theta} e^{-i\phi}
	\end{bmatrix} \begin{bmatrix}
		0&1\\
		1&0
	\end{bmatrix} \begin{bmatrix}
		\cos{\theta} e^{-i\phi}&-\sin{\theta}e^{i\psi}\\
		\sin{\theta}e^{-i\psi}&\cos{\theta} e^{i\phi}
	\end{bmatrix}\\
	=&  \begin{bmatrix}
		\sin{\theta}e^{i\psi} & \cos{\theta} e^{i\phi}\\
		\cos{\theta} e^{-i\phi}&-\sin{\theta}e^{-i\psi}
	\end{bmatrix} \begin{bmatrix}
		\cos{\theta} e^{-i\phi}&-\sin{\theta}e^{i\psi}\\
		\sin{\theta}e^{-i\psi}&\cos{\theta} e^{i\phi}
	\end{bmatrix}\\
	=& \begin{bmatrix}
		\cos\theta \sin\theta\big[e^{i(\psi-\phi)}+e^{i(\phi-\psi)}\big]&\cos^2\theta e^{2i\phi}-\sin^2\theta e^{2i\psi} \\
		\cos^2\theta e^{-2i\phi}-\sin^2\theta e^{-2i\psi}&-\cos\theta \sin\theta\big[e^{i(\psi-\phi)}+e^{i(\phi-\psi)}\big]
	\end{bmatrix} \numberthis \label{eq:U:sigma1:UT}
\end{align*}

The real part of the off diagonal elements of \eqref{eq:U:sigma1:UT} is:
\begin{align*}
	&\begin{bmatrix}
		0&\Re(\cos^2\theta e^{2i\phi}-\sin^2\theta e^{2i\psi}) \\
		\Re(\cos^2\theta e^{-2i\phi}-\sin^2\theta e^{-2i\psi})&0
	\end{bmatrix}\\
	=& \frac{1}{2}(\cos^2\theta e^{2i\phi}-\sin^2\theta e^{2i\psi}+ \cos^2\theta e^{-2i\phi}-\sin^2\theta e^{-2i\psi}) \sigma^1	\\
	=& \Re(x^2-y^2)	
\end{align*}

The imaginary part of the off diagonal elements of \eqref{eq:U:sigma1:UT} is:
\begin{align*}
	&\begin{bmatrix}
		0&\Im(\cos^2\theta e^{2i\phi}-\sin^2\theta e^{2i\psi}) \\
		\Im(\cos^2\theta e^{-2i\phi}-\sin^2\theta e^{-2i\psi})&0
	\end{bmatrix}\\
	=& \frac{1}{2}(\cos^2\theta e^{2i\phi}-\sin^2\theta e^{2i\psi}- \cos^2\theta e^{-2i\phi}+\sin^2\theta e^{-2i\psi}) \frac{\sigma^2}{i}	\\
	=& -\Im(x^2-y^2)	
\end{align*}

The diagonal elements of \eqref{eq:U:sigma1:UT} are:

\begin{align*}
	 \cos\theta \sin\theta\big[e^{i(\psi-\phi)}+e^{i(\phi-\psi)}\big]\begin{bmatrix}
		1&0\\
		0&-1
	\end{bmatrix}
	=& \cos\theta \sin\theta\big[e^{i(\psi-\phi)}+e^{i(\phi-\psi)}\big] \sigma^3 \text{, now}\\
	\cos\theta \sin\theta e^{i(\psi-\phi)}=& \cos\theta e^{-i\phi} \sin\theta e^{i\psi}\\
	=& \bar{x} y \text{, and}\\
	\cos\theta \sin\theta e^{i(\phi-\psi)}=& \cos\theta e^{i\phi} \sin\theta e^{-i\psi}\\
	=& \bar{x} y \text{, whence} \\
	\cos\theta \sin\theta\big[e^{i(\psi-\phi)}+e^{i(\phi-\psi)}\big] =& x\bar{y} + \bar{x}y\\
	=&2 \Re{x\bar{y}} \text{, and}\\
	\cos\theta \sin\theta\big[e^{i(\psi-\phi)}+e^{i(\phi-\psi)}\big] \sigma^3 =& 2 \Re({x\bar{y}}) \sigma^3 
\end{align*}

So \eqref{eq:U:sigma1:UT} becomes:
\begin{align*}
		U \sigma^1 U^T  =& \Re{(x^2-y^2)} \sigma^1 - \Im{(x^2-y^2)} \sigma^2 + 2 \Re({x\bar{y}}) \sigma^3 \numberthis \label{eq:U:sigma1:expanded}
\end{align*}

\begin{align*}
	U \sigma^2 U^T  =&  \begin{bmatrix}
		\cos{\theta} e^{i\phi}&\sin{\theta}e^{i\psi}\\
		-\sin{\theta}e^{-i\psi}&\cos{\theta} e^{-i\phi}
	\end{bmatrix} \begin{bmatrix}
		0&-i\\
		i&0
	\end{bmatrix} \begin{bmatrix}
		\cos{\theta} e^{-i\phi}&-\sin{\theta}e^{i\psi}\\
		\sin{\theta}e^{-i\psi}&\cos{\theta} e^{i\phi}
	\end{bmatrix}\\
	=&  i \begin{bmatrix}
		\cos{\theta} e^{i\phi}&\sin{\theta}e^{i\psi}\\
		-\sin{\theta}e^{-i\psi}&\cos{\theta} e^{-i\phi}
	\end{bmatrix} \begin{bmatrix}
		0&-1\\
		1&0
	\end{bmatrix} \begin{bmatrix}
		\cos{\theta} e^{-i\phi}&-\sin{\theta}e^{i\psi}\\
		\sin{\theta}e^{-i\psi}&\cos{\theta} e^{i\phi}
	\end{bmatrix}\\
	=&  i\begin{bmatrix}
		\sin{\theta}e^{i\psi}&-\cos{\theta} e^{i\phi}\\
		\cos{\theta} e^{-i\phi}&\sin{\theta}e^{-i\psi}
	\end{bmatrix} \begin{bmatrix}
		\cos{\theta} e^{-i\phi}&-\sin{\theta}e^{i\psi}\\
		\sin{\theta}e^{-i\psi}&\cos{\theta} e^{i\phi}
	\end{bmatrix}\\
   =& i \begin{bmatrix}
	   	\sin{\theta}e^{i\psi}\cos{\theta} e^{-i\phi}-\cos{\theta} e^{i\phi}\sin{\theta}e^{-i\psi}&-\sin^2{\theta}e^{2i\psi}-\cos^2{\theta} e^{2i\phi}\\
	   	\cos^2{\theta} e^{-2i\phi}+\sin^2{\theta}e^{-2i\psi}&-\cos{\theta} e^{-i\phi}\sin{\theta}e^{i\psi}+\sin{\theta}e^{-i\psi}\cos{\theta} e^{i\phi}
   \end{bmatrix} \\
	=& i \begin{bmatrix}
		\sin{\theta}\cos{\theta}\big[e^{i(\psi-\phi)}-e^{i(\phi-\psi)}\big]&-\sin^2{\theta}e^{2i\psi}-\cos^2{\theta} e^{2i\phi}\\
		\cos^2{\theta} e^{-2i\phi}+\sin^2{\theta}e^{-2i\psi}&\sin{\theta}\cos{\theta}\big[-e^{i(\psi-\phi)}+e^{i(\phi-\psi)}\big]
	\end{bmatrix} \numberthis \label{eq:U:sigma2:UT}
\end{align*}

The real part of the off diagonal terms in \eqref{eq:U:sigma2:UT} is:
\begin{align*}
	 &\begin{bmatrix}
		0&\Im(\sin^2{\theta}e^{2i\psi}+\cos^2{\theta} e^{2i\phi})\\
		-\Im(\cos^2{\theta} e^{-2i\phi}+\sin^2{\theta}e^{-2i\psi})&0
	\end{bmatrix}\\
   =& \begin{bmatrix}
		0&(\sin^2{\theta}\sin{2i\psi}+\cos^2{\theta} \sin{2i\phi})\\
		-(\cos^2{\theta} \sin({-2i\phi})+\sin^2{\theta}\sin({-2i\psi}))&0
	\end{bmatrix}\\
	=& \begin{bmatrix}
	0&(\sin^2{\theta}\sin{2i\psi}+\cos^2{\theta} \sin{2i\phi})\\
	(\cos^2{\theta} \sin({2i\phi})+\sin^2{\theta}\sin({2i\psi}))&0
	\end{bmatrix}\\
	=& (\sin^2{\theta}\sin{2i\psi}+\cos^2{\theta} \sin{2i\phi}) \sigma^1\\
	=& \Im(x^2 + y^2) \sigma^1
\end{align*}

The imaginary part of the off diagonal terms in \eqref{eq:U:sigma2:UT} is:
\begin{align*}
	\begin{bmatrix}
		0&-\Re({\sin^2{\theta}e^{2i\psi}+\cos^2{\theta} e^{2i\phi}})\\
		\Re({\cos^2{\theta} e^{-2i\phi}+\sin^2{\theta}e^{-2i\psi}})&0
	\end{bmatrix}
	=&\begin{bmatrix}
		0&-\Re(x^2+y^2)\\
		\Re(\bar{x}^2+\bar{y}^2)&0
	\end{bmatrix}\\
	=& \frac{\Re(x^2+y^2)}{i} \sigma_2
\end{align*}

The diagonal terms in \eqref{eq:U:sigma2:UT} are:
\begin{align*}
	i \sin{\theta}\cos{\theta}\big[e^{i(\psi-\phi)}-e^{i(\phi-\psi)}\big] \sigma^3 =& i \big[\bar{x}y-x\bar{y}\big] \sigma^3\\
	=&i 2 i  \Im({\bar{x}y}) \sigma^3\\
	=& - 2 \Im({\bar{x}y}) \sigma^3
\end{align*}

So \eqref{eq:U:sigma2:UT} becomes:
\begin{align*}
	U \sigma^2 U^T  =& \Im(x^2 + y^2) \sigma^1 + \Re(x^2+y^2) \sigma_2 - 2 \Im({\bar{x}y}) \sigma^3  \numberthis \label{eq:U:sigma2:expanded}
\end{align*}

\begin{align*}
	U \sigma^3 U^T =&  \begin{bmatrix}
		\cos{\theta} e^{i\phi}&\sin{\theta}e^{i\psi}\\
		-\sin{\theta}e^{-i\psi}&\cos{\theta} e^{-i\phi}
	\end{bmatrix} \begin{bmatrix}
		1&0\\
		0&-1
	\end{bmatrix} \begin{bmatrix}
		\cos{\theta} e^{-i\phi}&-\sin{\theta}e^{i\psi}\\
		\sin{\theta}e^{-i\psi}&\cos{\theta} e^{i\phi}
	\end{bmatrix}\\
	=& \begin{bmatrix}
		\cos{\theta} e^{i\phi}&-\sin{\theta}e^{i\psi}\\
		-\sin{\theta}e^{-i\psi}&-\cos{\theta} e^{-i\phi}
	\end{bmatrix}  \begin{bmatrix}
		\cos{\theta} e^{-i\phi}&-\sin{\theta}e^{i\psi}\\
		\sin{\theta}e^{-i\psi}&\cos{\theta} e^{i\phi}
	\end{bmatrix}\\
	=& \begin{bmatrix}
		\cos^2{\theta}-\sin^2{\theta}&-2 \cos{\theta}\sin{\theta}e^{i(\theta+\phi)}\\
		-2 \cos{\theta}\sin{\theta}e^{-i(\theta+\phi)}&-(\cos^2{\theta}-\sin^2{\theta})
	\end{bmatrix} \numberthis \label{eq:U:sigma3:UT}
\end{align*}
Now
\begin{align*}
	xy =& \cos{\theta} e^{i\phi} \sin{\theta} e^{i\psi}\\
	=& \cos{\theta} \sin{\theta}  e^{i(\phi + \psi)}\\
	=& \cos{\theta} \sin{\theta}  \big[\cos{(\phi + \psi)}+ i \sin{(\phi + \psi)}\big]\\
	=& \cos{\theta} \sin{\theta}  \big[\cos{[-(\phi + \psi)]}- i \sin{[-(\phi + \psi)]}\big]
\end{align*}
We see that the real part of the cross term in \eqref{eq:U:sigma3:UT} is:
\begin{align*}
	-2 \cos{\theta}\sin{\theta}\begin{bmatrix}
		0&\Re({e^{i(\phi + \psi)}})\\
		\Re({e^{-i(\phi + \psi)}})&0
	\end{bmatrix}=&	-2 \cos{\theta}\sin{\theta} \begin{bmatrix}
		0&\Re({e^{i(\phi + \psi)}})\\
		\Re({e^{-i(\phi + \psi)}})&0
	\end{bmatrix}\\
	=&	-2 \cos{\theta}\sin{\theta} \begin{bmatrix}
		.&\Re({e^{i(\phi + \psi)}})\\
		\Re({e^{i(\phi + \psi)}})&.\\
	\end{bmatrix} \\
	=& -2 \cos{\theta}\sin{\theta} \Re({e^{i(\phi + \psi)}}) \sigma^1\\
	=& 2 \Re(xy) \sigma^1
\end{align*}

Then the imaginary part of the cross term in \eqref{eq:U:sigma3:UT} is:
\begin{align*}
	-2 \cos{\theta}\sin{\theta}\begin{bmatrix}
		0&\Im({e^{i(\phi + \psi)}})\\
		\Im({e^{-i(\phi + \psi)}})&0
	\end{bmatrix}=&	-2 \cos{\theta}\sin{\theta} \begin{bmatrix}
		0&\Im({e^{i(\phi + \psi)}})\\
		-\Im({e^{i(\phi + \psi)}})&0\\
	\end{bmatrix} \\
	=& 2 \cos{\theta}\sin{\theta} \Im({e^{i(\phi + \psi)}}) \frac{\sigma^2}{i}\\
	=& 2 \Im(xy) \frac{\sigma^2}{i}
\end{align*}
Finally
\begin{align*}
	\vert x \vert^2 - \vert y \vert^2 =& \cos^2 \theta - \sin^2 \theta \text{, so the diagonal term in \eqref{eq:U:sigma3:UT} is}\\
	&(\vert x \vert^2 - \vert y \vert^2) \sigma^3
\end{align*}

So \eqref{eq:U:sigma3:UT} becomes:
\begin{align*}
		U \sigma^3 U^T =&  2 \Re(xy) \sigma^1 + 2 \Im(xy) \sigma^2 + (\vert x \vert^2 - \vert y \vert^2) \sigma^3 \numberthis \label{eq:U:sigma3:expanded}
\end{align*}

Collecting \eqref{eq:U:sigma1:expanded}, \eqref{eq:U:sigma2:expanded}, and \eqref{eq:U:sigma3:expanded}, we get:
\begin{equation}
	\begin{aligned}
		U \sigma^1 U^T  =& \Re{(x^2-y^2)} \sigma^1 -& \Im{(x^2-y^2)} \sigma^2 +& 2 \Re({x\bar{y}}) \sigma^3\\
		U \sigma^2 U^T  =& \Im(x^2 + y^2) \sigma^1 +& \Re(x^2+y^2) \sigma_2 -& 2 \Im({\bar{x}y}) \sigma^3  \\
		U \sigma^3 U^T =&  2 \Re(xy) \sigma^1 +& 2 \Im(xy) \sigma^2 +& (\vert x \vert^2 - \vert y \vert^2) \sigma^3
	\end{aligned}\label{eq:all3sigma}
\end{equation}

\section{Quantizing the Dirac Field}
\section{Lorentz Group and Weyl Spinors}

From \cite[II.3,(2,5,6)]{zee2010quantum}
\begin{align*}
	J_1 =& \begin{bmatrix}
		0&0&0&0\\
		0&0&0&0\\
		0&0&0&-i\\
		0&0&i&0\\
	\end{bmatrix}\;
	J_2 =& \begin{bmatrix}
		0&0&0&0\\
		0&0&0&i\\
		0&0&0&0\\
		0&-i&0&0\\
	\end{bmatrix}\;
	J_3 =& \begin{bmatrix}
		0&0&0&0\\
		0&0&-i&0\\
		0&i&0&0\\
		0&0&0&0\\
	\end{bmatrix} \numberthis \label{eq:Js}\\
	i K_1 =& \begin{bmatrix}
		0&1&0&0\\
		1&0&0&0\\
		0&0&0&0\\
		0&0&0&0\\
	\end{bmatrix}\;
	i K_2 =& \begin{bmatrix}
		0&0&1&0\\
		0&0&0&0\\
		1&0&0&0\\
		0&0&0&0\\
	\end{bmatrix}\;
	i K_3 =& \begin{bmatrix}
		0&0&0&1\\
		0&0&0&0\\
		0&0&0&0\\
		1&0&0&0\\
	\end{bmatrix} \numberthis \label{eq:Ks}
\end{align*}

\begin{thm}[$J_{+}$ and $J_{-}$ form two separate $SU(2)$ algebras]
	If we define:
	\begin{align*}
		J_{\pm i} \equiv & \frac{1}{2}\big(J_i\pm i K_i\big)\text{, then}\\
		\big[J_{\pm i},J_{\pm j}\big] =& i \epsilon_{ijk} J_{\pm k} \text{, and} \numberthis \label{eq:J:pm}\\
		\big[J_{+i},J_{-j}\big] =& 0 \numberthis \label{eq:J:pm1}
	\end{align*}
\end{thm}
\begin{proof}
	From \eqref{eq:Js}:
	\begin{align*}
		[J_1, J_2] =& \begin{bmatrix}
			0&0&0&0\\
			0&0&0&0\\
			0&-1&0&0\\
			0&0&0&0
		\end{bmatrix} - \begin{bmatrix}
							0&0&0&0\\
							0&0&-1&0\\
							0&0&0&0\\
							0&0&0&0\\
						\end{bmatrix}\\
		 =& \begin{bmatrix}
				0&0&0&0\\
				0&0&1&0\\
				0&-1&0&0\\
				0&0&0&0
			\end{bmatrix}\\
			=&i J_3
	\end{align*}
	
	From \eqref{eq:Ks}:
	\begin{align*}
		[K_1,K_2] =& -[i K_1, i K_2] \\
		=& [i K_2,i K_1] \\
		=& \begin{bmatrix}
			0&0&0&0\\
			0&0&0&0\\
			0&1&0&0\\
			0&0&0&0\\
		\end{bmatrix} -  \begin{bmatrix}
								0&0&0&0\\
								0&0&1&0\\
								0&0&0&0\\
								0&0&0&0\\
						 \end{bmatrix}\\
		 =&\begin{bmatrix}
			0&0&0&0\\
			0&0&-1&0\\
			0&1&0&0\\
			0&0&0&0\\
		\end{bmatrix}\\
		=& -i J_3 \text{, using \eqref{eq:Js}.}
	\end{align*}
	

	
	\begin{align*}
		\big[J_{+ i},	J_{+ j}\big]  = & \frac{1}{4}\big[J_i+ i K_i,J_j+ i K_j\big]\\
		 = & \frac{1}{4} \big[\big(J_i+ i K_i\big)\big(J_j+ i K_j\big)-\big(J_j+ i K_j\big)\big(J_i+ i K_i\big)\big]\\
		 = & \frac{1}{4} \big[J_iJ_j + i J_iK_j + iK_iJ_j - K_iK_j - J_jJ_i - i J_j K_i -i K_j J_i +K_jK_i\big]\\
		 = & \frac{1}{4} \big[[J_i,J_j] - [K_i,K_j] + i[J_i,K_j]-i[J_j,K_i] \big] \\
		 = & \frac{1}{4} \big[i\epsilon_{ijk}J_k +i\epsilon_{ijk}J_k + i^2\epsilon_{ijk}K_k-i^2\epsilon_{jik}K_k] \big]\\
		 =& \frac{i}{2} \big[\epsilon_{ijk}J_k+i \epsilon_{ijk}K_k\big]\\
		 =& \frac{i}{2} \epsilon_{ijk}J_{+ k}
	\end{align*}
	
	Which is the $+$ case of \eqref{eq:J:pm}. Define
	\begin{align*}
		K_i^\prime =& - K_i\\
		J_{+i}^\prime =& J_i +  K_i^\prime
	\end{align*}
	We see that the argument for \eqref{eq:J:pm} suffices to establish:
	\begin{align*}
		\big[J_{+ i}^\prime, J_{+ j}^\prime\big] =&  \frac{i}{2} \epsilon_{ijk}J_{+ k} ^\prime \text{, but}\\
		J_{+i}^\prime =& J_{-i}\text{, whence}\\
		\big[J_{- i}, J_{- j} \big] =&  \frac{i}{2} \epsilon_{ijk}J_{- k}
	\end{align*}
	Which is the $-$ case of \eqref{eq:J:pm}. Finally:
	\begin{align*}
		\big[J_{+ i},	J_{- j}\big]  = & \frac{1}{4}\big[J_i+ i K_i,J_j- i K_j\big]\\
		= & \frac{1}{4} \big[\big(J_i+ i K_i\big)\big(J_j- i K_j\big)-\big(J_j- i K_j\big)\big(J_i+ i K_i\big)\big]\\
		= & \frac{1}{4} \big[J_iJ_j -i J_iK_j +iK_iJ_j+K_iK_j - J_jJ_i -iJ_j K_i+iK_jJ_i-K_jK_i\big] \\
		= & \frac{1}{4} \big[[J_i,J_j] +[K_i,K_j]  -i[J_i,K_j] +i \underbrace{[K_i,J_j]}_\text{$-[J_j,K_i]$}\big] \\
		= & \frac{1}{4} \big[\cancel{i\epsilon_{ijk}J_k} - \cancel{i\epsilon_{ijk}J_k} -\bcancel{i^2\epsilon_{ijk}K_k} -\bcancel{i^2\epsilon_{jik}K_k}\big]\\
		=& 0
	\end{align*}
	Which establishes \eqref{eq:J:pm1}.
\end{proof}

\section{Spin-Statistics Connection}
\section{Vacuum Energy, Grassman Integrals, and Feynman Diagrams for Fermions}
\section{Electron Scattering and Gauge Invariance}
\section{Diagrammatic Proof of Gauge Invariance}
\section{Photon-Electron Scattering}

\bibliographystyle{unsrt}
\addcontentsline{toc}{section}{Bibliography}
\raggedright
\bibliography{tm}

\end{document}
